Save.

src/FJ/condensed/FJ.v
@@ -361,10 +361,7 @@ Module CTSanity.
 (* The freely generated relation must have Object as all the possible top,
   however, must be well-defined classes
   *)
-Hypothesis obj_sub_all: 
-  forall C D Fs noDupfs K Ms noDupMds,
-  find C CT = Some (CDecl C D Fs noDupfs K Ms noDupMds) ->
-  C <: Object.
+
 Hypothesis obj_notin_dom: find Object CT = None.
 Hint Rewrite obj_notin_dom.
 
@@ -410,22 +407,101 @@ Proof.
 Qed.
 
 
-(* This following is purely wrong, 
-  recall ClassName = id, so it is impossible we can find   *)
-(* Lemma subtype_wf: forall D,
-  D <> Object ->
-  exists E Fs noDupfs K Ms noDupMds, D <: E /\ find E CT = Some (CDecl E Object Fs noDupfs K Ms noDupMds).
-Proof.
-  intros. assert (D <: Object) by (exact (obj_sub_all D)).
-  remember Object. gen H. gen Heqc. induction H0; intros; subst.
-  false. apply H. reflexivity. destruct beq_id_dec with D Object.
-  subst. eapply IHSubtype1; auto.
-  subst. destruct IHSubtype2; auto. do 6 destruct H0.
-  exists x. do 5 eexists; split; eauto.
-  exists C; do 5 eexists; split; eauto.
-Qed. *)
 
 Module subtype_dec.
+(* A more proof-relevant subtype *)
+Inductive nSubtype : [ClassName] -> ClassName -> ClassName -> Prop :=
+  | nS_Refl: forall C: ClassName, nSubtype (C :: nil) C C
+  | nS_Decl: forall C D E fs noDupfs K mds noDupMds trace,
+    find C CT = Some (CDecl C D fs noDupfs K mds noDupMds ) ->
+    nSubtype trace D E ->
+    nSubtype (C::trace) C E.
+
+Hint Constructors nSubtype.
+
+Lemma nSubtype__Subtype:
+  forall A B trace,
+    nSubtype trace A B -> Subtype A B.
+intros A B trace h.
+induction h; intros; subst; eauto.
+Qed.
+
+Lemma nSubtype_trans:
+  forall {A B t1},
+  nSubtype t1 A B ->
+    forall {C t2},
+    nSubtype t2 B C ->
+    exists t, nSubtype t A C.
+  intros A B t1 h.
+  induction h; intros; subst; eauto.
+  destruct (IHh _ _ H0).  eauto.
+Qed. 
+
+Lemma Subtype__nSubtype:
+  forall A B,
+  A <: B -> (exists trace, nSubtype trace A B).
+intros A B h. induction h; intros; subst; eauto.
+destruct IHh1 as [t1 hh1].
+destruct IHh2 as [t2 hh2].
+forwards*: (nSubtype_trans hh1 hh2).
+Qed.
+
+
+
+Theorem nSubtype_unique':
+  forall A B t1, 
+    nSubtype t1 A B ->
+    forall C t2,
+    nSubtype t2 A C ->
+    t1 = t2.
+intros A B t1 h.
+induction h; intros; subst; eauto.
+admit.
+induction H0; intros; subst; eauto. 
+
+Theorem nSubtype_unique:
+  forall A B t1 t2, 
+    nSubtype t1 A B ->
+    nSubtype t2 A B ->
+    t1 = t2.
+intros A B t1 t2 h1. generalize dependent t2.
+induction h1; intros; subst; eauto.
+
+admit. inversion H; subst; eauto.  
+
+
+
+Parameter nSubtype_trace:
+  forall A,
+    find A CT <> None -> 
+    exists t, nSubtype t A Object.
+
+Lemma nSubtype_trace1:
+  forall A B t,
+    A <: B -> nSubtype t A Object -> In B t.
+(* Use uniqueness, since B <: Object *)
+Admitted.
+
+Lemma nSubtype_trace2:
+  forall A B t,
+    nSubtype t A Object -> In B t -> exists t', nSubtype t' A B.
+Admitted.
+
+Lemma dec_subtype': forall C,
+  find C CT <> None ->
+  forall D,
+  decidable (Subtype C D).
+unfold decidable.
+intros C h. destruct (nSubtype_trace C h) as [tr hh].
+intros D.
+(* Now we check if D is in tr *)
+edestruct (in_dec beq_id_dec D tr).
+destruct (nSubtype_trace2 C D tr); eauto. left. eapply nSubtype__Subtype; eauto.
+right; intros H. forwards*: (nSubtype_trace1 C D tr).
+Qed.
+
+Lemma nonexistent_
+
 
 End subtype_dec.
 
